PRFs

examples/low-level/crypto/Crypto.Symmetric.PRF.fst
@@ -106,7 +106,7 @@ noextract let find (#rgn:region) (#i:id) (s:table rgn i) (x:domain i) : option (
   match SeqProperties.find_l (is_entry_domain x) s with
   | Some e -> Some e.range
   | None   -> None
-  
+
 let find_sk0 #rgn (#i:id) s (x:domain_sk0 i) = 
   match find s x with
   | Some v -> Some(sk0Range rgn i x v)
@@ -124,43 +124,12 @@ let find_blk #rgn (#i:id) s (x:domain_blk i) =
   | Some v -> Some (blkRange rgn i x v)
   | None   -> None
 
-//16-12-19 imported from Crypto.AEAD.Invariant
-
-let lemma_find_append_some
-  (#r:region)
-  (#i:id)
-  (table0:table r i)
-  (table1:table r i)
-  (x:domain i) 
-  : Lemma
-    (requires (Some? (find table0 x)))
-    (ensures  (find (Seq.append table0 table1) x == find table0 x))
-  = SeqProperties.find_append_some table0 table1 (is_entry_domain x)
-
-let lemma_find_append_some_forall
-  (#r:region)
-  (#i:id)
-  (table0:table r i)
-  (table1:table r i) : 
-  Lemma 
-    (ensures 
-	(forall (x:domain i).{:pattern (find (Seq.append table0 table1) x) }
-	   Some? (find table0 x) ==>
-	   find (Seq.append table0 table1) x == find table0 x))
- = let open FStar.Classical in
-   forall_intro (move_requires (lemma_find_append_some #r #i table0 table1))
-
-let lemma_find_append_none
-  (#r:region)
-  (#i:id)
-  (table0:table r i)
-  (table1:table r i)
-  (x:PRF.domain i) 
-  : Lemma
-    (requires (None? (find table1 x)))
-    (ensures  (find (Seq.append table0 table1) x == find table0 x))
-  = SeqProperties.find_append_none_s2 table0 table1 (is_entry_domain x)
-
+(* not sure why it fails; inlined below.
+#reset-options "--z3rlimit 100"
+private val lemma_find_snoc: #rgn:region -> #i:id -> s:table rgn i -> e:entry rgn i -> Lemma (ensures (find (SeqProperties.snoc s e) e.x == Some e.range))
+let lemma_find_snoc #rgn #i s e = 
+  SeqProperties.find_snoc s e (is_entry_domain e.x)
+*)
 
 
 // The table exists only for idealization
@@ -265,7 +234,7 @@ val prf_mac:
       let r = itable i t in
       let t0 = HS.sel h0 r in
       let t1 = HS.sel h1 r in
-      (forall (y:domain i). y <> x ==> find t0 y == find t1 y)  /\ //at most modifies t at x
+      //16-12-20 now proved in AEAD: (forall (y:domain i). y <> x ==> find t0 y == find t1 y)  /\ //at most modifies t at x
       (match find_mac (HS.sel h0 r) x with // already in the table? 
        | Some mc' -> 
            h0 == h1 /\ // when decrypting
@@ -282,7 +251,6 @@ val prf_mac:
               HS.modifies_transitively (Set.singleton t.rgn) h0 h1 /\
               HS.modifies_ref t.rgn !{HS.as_ref r} h0 h1 /\
 	 HS.modifies_ref t.mac_rgn TSet.empty h0 h1
-              //16-10-11 we miss a more precise clause capturing the table update   
           | None -> False ))
     else (
       CMA.genPost (i,x.iv) t.mac_rgn h0 mc h1 /\
@@ -294,10 +262,9 @@ val prf_mac:
 #reset-options "--z3rlimit 100"
 
 let prf_mac i t k_0 x =
-  let h0 = get () in
-  assume(CMA.skeyed i ==> Buffer.live h0 (CMA.get_skey #t.mac_rgn #i k_0));// TODO move to precondition
   Buffer.recall t.key;
   recall_region t.mac_rgn;
+  if CMA.skeyed i then Buffer.recall (CMA.get_skey #t.mac_rgn #i k_0);
   let macId = (i,x.iv) in
   if prf i then
     begin
@@ -306,23 +273,15 @@ let prf_mac i t k_0 x =
     let contents = !r in
     match find_mac contents x with
     | Some mc ->  (* beware: mac shadowed by CMA.mac *)
-        assume false;
-        (* 
-        assume (CMA.(MAC.norm h0 mc.r)); //TODO: replace this using monotonicity
-        assume (HS.(Buffer.(CMA.(not ((Buffer.content mc.s).mm))))); //TODO: mark this as not manually managed
+        let h0 = ST.get() in
+        assume (CMA.(MAC.norm h0 mc.r)); //16-12-20 TODO: replace this using monotonicity
         Buffer.recall (CMA.(mc.s));
-        mc
-        *)
+        if mac_log then FStar.Monotonic.RRef.m_recall (CMA.(ilog mc.log));
         mc
     | None ->
         let mc = CMA.gen t.mac_rgn macId k_0 in
         r := SeqProperties.snoc contents (Entry x mc);
-        let h1 = ST.get() in 
-        assume(
-          let t0 = HS.sel h0 r in
-          let t1 = HS.sel h1 r in
-          find_mac t1 x == Some mc /\
-          (forall (y:domain i). y <> x ==> find t0 y == find t1 y));
+        SeqProperties.find_snoc contents (Entry x mc) (is_entry_domain x);
         mc
     end
   else
@@ -344,17 +303,18 @@ val prf_sk0:
       let r = itable i t in
       let t0 = HS.sel h0 r in
       let t1 = HS.sel h1 r in
-      (forall (y:domain i). y <> x ==> find t0 y == find t1 y)  /\ //at most modifies t at x
+      //now proved in AEAD: (forall (y:domain i). y <> x ==> find t0 y == find t1 y)  /\ //at most modifies t at x
       Buffer.live h1 k /\ 
       (match find_sk0 #t.mac_rgn #i (HS.sel h0 r) x with // already in the table? 
        | Some r0 -> k == r0 /\ h0 == h1
        | None ->  
          (match find_sk0 (HS.sel h1 r) x with 
-          | Some r1 -> k == r1 /\
-	    t1 == SeqProperties.snoc t0 (Entry x r1) /\
-            HS.modifies_transitively (Set.singleton t.rgn) h0 h1 /\
-            HS.modifies_ref t.rgn !{HS.as_ref r} h0 h1 /\
-	    HS.modifies_ref t.mac_rgn TSet.empty h0 h1
+          | Some r1 -> 
+              k == r1 /\
+              t1 == SeqProperties.snoc t0 (Entry x r1) /\
+              HS.modifies_transitively (Set.singleton t.rgn) h0 h1 /\
+              HS.modifies_ref t.rgn !{HS.as_ref r} h0 h1 /\
+              HS.modifies_ref t.mac_rgn TSet.empty h0 h1
           | None -> False ))
     else (
       Buffer.live h1 k /\
@@ -374,11 +334,9 @@ let prf_sk0 #i t =
       | None -> 
           let sk0 = CMA.get_skey (CMA.akey_gen t.mac_rgn i) in
           r := SeqProperties.snoc contents (Entry x sk0);
+          SeqProperties.find_snoc contents (Entry x sk0) (is_entry_domain x);
           sk0 in
-      assume (HS.is_eternal_region t.mac_rgn);
-      assume (HS.(Buffer.(CMA.(not ((Buffer.content sk0).mm))))); //TODO: mark this as not manually managed
       Buffer.recall sk0;
-      assume false; //NS: disovered while triaging this file ... unable to prove that (find_sk0 (HS.sel h1 r) x = Some _)
       sk0
     end
   else
@@ -534,13 +492,6 @@ let prf_dexor i t x l cipher plain =
 ////////////////////////////////////////////////////////////////////////////////
 
 
-#set-options "--initial_fuel 1 --max_fuel 1"
-
-private let lemma_snoc_found (#rgn:region) (#i:id) (s:Seq.seq (entry rgn i)) (x:domain i) (v:range rgn i x) : Lemma
-  (requires (find s x == None))
-  (ensures (find (SeqProperties.snoc s (Entry x v)) x == Some v))
-  = admit() //TODO, move this ... find_append_r
-
 #reset-options "--z3rlimit 100"
 
 // generates a fresh block for x and XORs it with plaintext
@@ -573,9 +524,7 @@ let prf_enxor i t x l cipher plain =
     let c = random_bytes l in // sample a fresh ciphertext block
     let newblock = OTP #i l p c in
     let contents' = SeqProperties.snoc contents (Entry x newblock) in
-    lemma_snoc_found contents x newblock;
-    assert(find_otp #t.mac_rgn #i contents x == None); 
-    assert(find_otp #t.mac_rgn #i contents' x == Some newblock);
+    SeqProperties.find_snoc contents (Entry x newblock) (is_entry_domain x);
 
     let h0 = ST.get() in
     assert(p == sel_plain h0 l plain);
